\documentclass[main.tex]{subfiles}

\begin{document}

\section{Aufgabe 2}
Berechnen Sie die folgenden Dreifachintegrale:
\begin{enumerate}
\item 
$\begin{aligned}
\int \limits_{x=0}^{1} 
	\int \limits_{y=0}^{1-x} 
		\int \limits_{z=0}^{2-x} x \cdot y \cdot z \ dz \ dy \ dx
\end{aligned}$
\item 
$\begin{aligned}
\int \limits_{\alpha=0}^{\frac{\pi}{2}} 
	\int \limits_{r=0}^{1} 
		\int \limits_{z=0}^{2} 
			z \cdot r^2 \cdot \sin(\alpha) \ dz \ dr \ d\alpha
\end{aligned}$
\end{enumerate}

\subsection{Lösung 2a}

\begin{align*}
    \int \limits_{x=0}^{1} 
	\int \limits_{y=0}^{1-x} 
    \int \limits_{z=0}^{2-x} x \cdot y \cdot z \dx{(z,y,x)}
 &= \int \limits_{x=0}^{1} 
    \int \limits_{y=0}^{1-x} 
    \left[ \frac{x \cdot y}{2} \cdot z^2 \right]_{z=0}^{2-x} \dx{(y,x)} \\
 &= \int \limits_{x=0}^{1} 
    \int \limits_{y=0}^{1-x} 
    \frac{1}{2} \cdot x \cdot y \cdot (2-x)^2 \dx{(y,x)} \\
 &= \int \limits_{x=0}^{1} 
    \left[ \frac{1}{4} \cdot x \cdot (2-x)^2 \cdot y^2 \right]_{y=0}^{1-x} \dx{x} \\
 &= \int \limits_{0}^{1} \frac{1}{4} \cdot x \cdot (2-x)^2 \cdot (1-x)^2 \dx{x} \\
 &= \int \limits_{0}^{1} \frac{1}{4} x^5 - \frac{3}{2} x^4 + \frac{13}{4} x^3 - 3 x^2 + x \dx{x} \\
 &= \left[ \frac{1}{24} x^6 - \frac{3}{10} x^5 + \frac{13}{16} x^4 - x^3 + \frac{1}{2}x^2 \right]_{0}^{1} \\
 &= \frac{1}{24} - \frac{3}{10} + \frac{13}{16} - 1 + \frac{1}{2} \\[2mm]
 &= \frac{13}{240} \\
\end{align*}

\subsection{Lösung 2b}

\begin{align*}
    \int \limits_{\alpha=0}^{\frac{\pi}{2}} 
	\int \limits_{r=0}^{1} 
    \int \limits_{z=0}^{2} 
        z \cdot r^2 \cdot \sin(\alpha) 
    \dx{(z, r, \alpha)}
    &=
    \int \limits_{\alpha=0}^{\frac{\pi}{2}} 
	\int \limits_{r=0}^{1} 
        \left[ \frac{1}{2} r^2 \cdot \sin(\alpha) \cdot z^2 \right]_{z=0}^{2}  
    \dx{(r, \alpha)} \\
    &=
    \int \limits_{\alpha=0}^{\frac{\pi}{2}} 
	\left[ 
        \frac{1}{6} r^3 \cdot \sin(\alpha) \cdot 4  
    \right]_{r=0}^{1}
    \dx{\alpha} \\
    &=
    \int \limits_{\alpha=0}^{\frac{\pi}{2}} 
        \frac{4}{6} \sin(\alpha)  
    \dx{\alpha} \\
    &= \left[ - \frac{2}{3} \cos(\alpha) \right]_{\alpha=0}^{\frac{\pi}{2}} \\
    &= - \frac{2}{3} \cos\left(\frac{\pi}{2}\right) + \frac{2}{3} \cos(0)  \\
    &=  \frac{2}{3} \\
\end{align*}

\end{document}
